bedrock2/src/bedrock2/LeakageLoops.v
@@ -1,7 +1,7 @@
-Require Import List.
+From Coq Require Import List.
 Import ListNotations.
 Require Import coqutil.Datatypes.PrimitivePair coqutil.Datatypes.HList coqutil.dlet.
-Require Import Coq.Classes.Morphisms BinIntDef.
+From Coq Require Import Classes.Morphisms BinIntDef.
 Require Import coqutil.Macros.unique coqutil.Map.Interface coqutil.Word.Interface. Import map.
 Require Import coqutil.Word.Bitwidth.
 Require Import coqutil.Map.Properties.
